Skeletons are super simple now.

skeletons/skeleton_lemmas.v
@@ -19,103 +19,20 @@ apply skeletons_ignore_csubtype in H. auto.
 Qed.
 
 
-Fixpoint has_vtype_annotates Γ v A (types : has_vtype Γ v A):
-  exists v', v_ann Γ v A types v'
-with has_ctype_annotates Γ c C (types : has_ctype Γ c C):
-  exists c', c_ann Γ c C types c'
-with has_htype_annotates Γ h Σ D (types : has_htype Γ h Σ D):
-  exists h', h_ann Γ h Σ D types h'.
-{
-rename has_vtype_annotates into VL.
-rename has_ctype_annotates into CL.
-rename has_htype_annotates into HL.
-destruct types. destruct h.
-+ eexists. apply AnnUnit.
-+ eexists. apply AnnInt.
-+ eexists. apply AnnVar. auto.
-+ specialize (VL _ _ _ h) as IH1. destruct IH1 as [v1' ann1].
-  specialize (VL _ _ _ h0) as IH2. destruct IH2 as [v2' ann2].
-  eexists. eapply AnnPair; eauto.
-+ specialize (VL _ _ _ h) as IH1. destruct IH1 as [v' ann1].
-  eexists. eapply AnnLeft; eauto.
-+ specialize (VL _ _ _ h) as IH1. destruct IH1 as [v' ann1].
-  eexists. eapply AnnRight; eauto. 
-+ eexists. apply AnnNil.
-+ specialize (VL _ _ _ h) as IH1. destruct IH1 as [v1' ann1].
-  specialize (VL _ _ _ h0) as IH2. destruct IH2 as [v2' ann2].
-  eexists. eapply AnnCons; eauto.
-+ specialize (CL _ _ _ h) as IH1. destruct IH1 as [c' ann1].
-  eexists. eapply AnnFun; eauto.
-+ specialize (CL _ _ _ h0) as IH1. destruct IH1 as [c' ann1].
-  specialize (HL _ _ _ _ h1) as IH2. destruct IH2 as [h' ann2].
-  eexists. eapply AnnHandler; eauto.
-+ specialize (VL _ _ _ h) as IH1. destruct IH1 as [v1' ann1].
-  eexists. eapply AnnVSTy; eauto.
-}{
-rename has_vtype_annotates into VL.
-rename has_ctype_annotates into CL.
-rename has_htype_annotates into HL.
-destruct types. destruct h.
-+ specialize (VL _ _ _ h) as IH1. destruct IH1 as [v1' ann1].
-  eexists. eapply AnnRet; eauto.
-+ specialize (VL _ _ _ h) as IH1. destruct IH1 as [v1' ann1].
-  eexists. eapply AnnAbsurd; eauto.
-+ specialize (VL _ _ _ h) as IH. destruct IH as [v' ann].
-  specialize (CL _ _ _ h0) as IH1. destruct IH1 as [c1' ann1].
-  eexists. eapply AnnProdMatch; eauto.
-+ specialize (VL _ _ _ h) as IH. destruct IH as [v' ann].
-  specialize (CL _ _ _ h0) as IH1. destruct IH1 as [c1' ann1].
-  specialize (CL _ _ _ h1) as IH2. destruct IH2 as [c2' ann2].
-  eexists. eapply AnnSumMatch; eauto.
-+ specialize (VL _ _ _ h) as IH. destruct IH as [v' ann].
-  specialize (CL _ _ _ h0) as IH1. destruct IH1 as [c1' ann1].
-  specialize (CL _ _ _ h1) as IH2. destruct IH2 as [c2' ann2].
-  eexists. eapply AnnListMatch; eauto.
-+ specialize (CL _ _ _ h) as IH1. destruct IH1 as [c1' ann1].
-  specialize (CL _ _ _ h0) as IH2. destruct IH2 as [c2' ann2].
-  eexists. eapply AnnDo; eauto.
-+ specialize (VL _ _ _ h) as IH1. destruct IH1 as [v1' ann1].
-  specialize (VL _ _ _ h0) as IH2. destruct IH2 as [v2' ann2].
-  eexists. eapply AnnApp; eauto.
-+ specialize (VL _ _ _ h) as IH1. destruct IH1 as [v1' ann1].
-  specialize (CL _ _ _ h0) as IH2. destruct IH2 as [c2' ann2].
-  eexists. eapply AnnHandle; eauto.
-+ specialize (CL _ _ _ h) as IH1. destruct IH1 as [c1' ann1].
-  specialize (CL _ _ _ h0) as IH2. destruct IH2 as [c2' ann2].
-  eexists. eapply AnnLetRec; eauto.
-+ specialize (VL _ _ _ h) as IH1. destruct IH1 as [v1' ann1].
-  specialize (CL _ _ _ h0) as IH2. destruct IH2 as [c2' ann2].
-  eexists. eapply AnnOp; eauto.
-+ specialize (CL _ _ _ h) as IH1. destruct IH1 as [c1' ann1].
-  eexists. eapply AnnCSTy; eauto.
-}{
-rename has_vtype_annotates into VL.
-rename has_ctype_annotates into CL.
-rename has_htype_annotates into HL.
-destruct types. destruct h0.
-+ eexists. eapply AnnCasesØ.
-+ specialize (HL _ _ _ _ h0) as IH1. destruct IH1 as [c' ann1].
-  specialize (CL _ _ _ h1) as IH2. destruct IH2 as [h' ann2].
-  eexists. eapply AnnCasesU; eauto.
-}
-Qed.
-
-
-Fixpoint ann_val_types Γ v A (types : has_vtype Γ v A) v'
-  (ann: v_ann Γ v A types v') {struct ann}:
-  has_sk_vtype 
-    (skeletize_ctx Γ) v' (skeletize_vtype A)
-with ann_comp_types Γ c C (types : has_ctype Γ c C) c'
-  (ann: c_ann Γ c C types c') {struct ann}:
-  has_sk_ctype 
-    (skeletize_ctx Γ) c' (skeletize_ctype C)
-with ann_hcases_types Γ h Σ D (types : has_htype Γ h Σ D) h'
-  (ann: h_ann Γ h Σ D types h') {struct ann}:
-  has_sk_htype 
-    (skeletize_ctx Γ) h' (skeletize_ctype D).
+Fixpoint skeleton_val_type Γ v A (types : has_vtype Γ v A) {struct types}:
+  has_sk_vtype (skeletize_ctx Γ) (skeletize_val v) (skeletize_vtype A)
+with skeleton_comp_type Γ c C (types : has_ctype Γ c C) {struct types}:
+  has_sk_ctype (skeletize_ctx Γ) (skeletize_comp c) (skeletize_ctype C)
+with skeleton_hcases_type Γ h Σ D (types : has_htype Γ h Σ D) {struct types}:
+  has_sk_htype (skeletize_ctx Γ) (skeletize_hcases h) (skeletize_ctype D).
 Proof.
+all: rename skeleton_val_type into VL.
+all: rename skeleton_comp_type into CL.
+all: rename skeleton_hcases_type into HL.
 {
-destruct ann; simpl.
+destruct types. destruct H1; simpl.
++ apply SkTypeUnit.
++ apply SkTypeInt.
 + apply SkTypeVar.
   assert (forall n γ A, get_vtype γ n = Some A ->
     get_sk_vtype (skeletize_ctx γ) n = Some (skeletize_vtype A)).
@@ -123,466 +40,52 @@ destruct ann; simpl.
     destruct k. 
     + simpl in gets. inv gets. auto.
     + simpl in *. auto. }
-  apply H0. auto.
-+ apply SkTypeUnit.
-+ apply SkTypeInt.
+  apply H2. auto.
 + apply SkTypePair; eauto.
 + apply SkTypeLeft; eauto.
 + apply SkTypeRight; eauto.
 + apply SkTypeNil.
-+ apply SkTypeCons; eauto.
-  eapply ann_val_types in ann2. simpl in *. auto.
-+ apply SkTypeFun.
-  eapply ann_comp_types in H. simpl in *. auto.
-+ apply SkTypeHandler.
-  eapply ann_comp_types in H. simpl in *. auto.
-  eapply ann_hcases_types in H0. simpl in *. auto.
-+ eapply ann_val_types in ann. simpl in *.
-  apply skeletons_ignore_vsubtype in H. inv H. auto.
++ apply SkTypeCons; eauto. apply VL in H2. simpl in *. auto.
++ apply SkTypeFun. eapply CL in H1. simpl in *. auto.
++ apply SkTypeHandler. 
+  eapply CL in H1. simpl in *. auto.
+  eapply HL in H2. simpl in *. auto.
++ eapply VL in H1. simpl in *.
+  apply skeletons_ignore_vsubtype in H2. inv H2. auto.
 }{
-destruct ann; simpl.
+destruct types. destruct H1; simpl.
 + apply SkTypeRet. eauto.
-+ apply SkTypeAbsurd.
-  eapply ann_val_types in H. simpl in *. auto.
++ apply SkTypeAbsurd. eapply VL in H1. simpl in *. auto.
 + eapply SkTypeProdMatch.
-  eapply ann_val_types in H. simpl in *. eauto.
-  eapply ann_comp_types in ann. simpl in *. auto.
+  eapply VL in H1. simpl in *. eauto.
+  eapply CL in H2. simpl in *. auto.
 + eapply SkTypeSumMatch.
-  eapply ann_val_types in H. simpl in *. eauto.
-  eapply ann_comp_types in ann1. simpl in *. auto.
-  eapply ann_comp_types in ann2. simpl in *. auto.
+  eapply VL in H1. simpl in *. eauto.
+  eapply CL in H2. simpl in *. auto.
+  eapply CL in H3. simpl in *. auto.
 + eapply SkTypeListMatch.
-  eapply ann_val_types in H. simpl in *. eauto.
-  eapply ann_comp_types in ann1. simpl in *. auto.
-  eapply ann_comp_types in ann2. simpl in *. auto.
+  eapply VL in H1. simpl in *. eauto.
+  eapply CL in H2. simpl in *. auto.
+  eapply CL in H3. simpl in *. auto.
 + eapply SkTypeDo.
-  eapply ann_comp_types in ann1. simpl in *. eauto.
-  eapply ann_comp_types in ann2. simpl in *. auto.
+  eapply CL in H1. simpl in *. eauto.
+  eapply CL in H2. simpl in *. auto.
 + eapply SkTypeApp; eauto.
-  eapply ann_val_types in H. simpl in *. auto.
+  eapply VL in H1. simpl in *. auto.
 + eapply SkTypeHandle; eauto.
-  eapply ann_val_types in H. simpl in *. auto.
+  eapply VL in H1. simpl in *. auto.
 + eapply SkTypeLetRec.
-  eapply ann_comp_types in ann1. simpl in *. eauto.
-  eapply ann_comp_types in ann2. simpl in *. auto.
+  eapply CL in H1. simpl in *. eauto.
+  eapply CL in H2. simpl in *. auto.
 + eapply SkTypeOp. eauto.
-  eapply ann_comp_types in ann. simpl in *. auto.
-+ eapply ann_comp_types in ann. simpl in *.
-  apply skeletons_ignore_csubtype in H. inv H. auto.
+  eapply CL in H7. simpl in *. auto.
++ eapply CL in H1. simpl in *.
+  apply skeletons_ignore_csubtype in H2. inv H2. auto.
 }{
-destruct ann; simpl.
+destruct types. destruct H2; simpl.
 + apply SkTypeCasesØ.
 + eapply SkTypeCasesU. eauto.
-  eapply ann_comp_types in H. simpl in *. auto.
+  eapply CL in H3. simpl in *. auto.
 }
 Qed.
 
-
-(* Due to subtyping we need manual inversion :( *)
-
-Fixpoint inv_ann_Var Γ n A p v'
-  (ann: v_ann Γ (Var n) A p v'):
-  v' = SkVar n.
-Proof.
-inv ann. auto. apply inv_ann_Var in H. auto.
-Qed.
-
-Fixpoint inv_ann_Unit Γ A p v'
-  (ann: v_ann Γ Unit A p v'):
-  v' = SkUnit.
-Proof.
-inv ann. auto. apply inv_ann_Unit in H. auto.
-Qed.
-
-Fixpoint inv_ann_Int Γ n A p v'
-  (ann: v_ann Γ (Int n) A p v'):
-  v' = SkInt n.
-Proof.
-inv ann. auto. apply inv_ann_Int in H. auto.
-Qed.
-
-Fixpoint inv_ann_Pair Γ v1 v2 A B p v'
-  (ann: v_ann Γ (Pair v1 v2) (TyProd A B) p v') {struct ann}:
-  exists v1' v2' A' B' p1 p2,
-    vsubtype A' A /\ vsubtype B' B /\
-    v_ann Γ v1 A' p1 v1' /\ v_ann Γ v2 B' p2 v2' /\
-    v' = SkPair v1' v2'.
-Proof.
-inv ann.
-+ exists v1', v2', A, B, p1, p2. aconstructor. 2: aconstructor.
-  all: apply vsubtype_refl; inv p; inv H0; auto.
-+ inv H0. eapply inv_ann_Pair in H.
-  destruct H as [v1'[v2'[A'[B'[p1[p2[stya[styb othr]]]]]]]].
-  exists v1',v2',A',B',p1,p2.
-  do 2 try aconstructor.
-  all: eapply vsubtype_trans; eauto.
-Qed.
-
-Fixpoint inv_ann_Left Γ v A B p v'
-  (ann: v_ann Γ (Left v) (TySum A B) p v') {struct ann}:
-  exists v1' A' p1,
-    vsubtype A' A /\ v_ann Γ v A' p1 v1' /\ v' = SkLeft v1'.
-Proof.
-inv ann.
-+ exists v'0, A, pl. aconstructor.
-  apply vsubtype_refl. inv p. inv H0. auto.
-+ inv H0. eapply inv_ann_Left in H.
-  destruct H as [v1'[A'[p1[stya othr]]]].
-  exists v1',A',p1. aconstructor.
-  eapply vsubtype_trans; eauto.
-Qed.
-
-Fixpoint inv_ann_Right Γ v A B p v'
-  (ann: v_ann Γ (Right v) (TySum A B) p v') {struct ann}:
-  exists v1' B' p1,
-    vsubtype B' B /\ v_ann Γ v B' p1 v1' /\ v' = SkRight v1'.
-Proof.
-inv ann.
-+ exists v'0, B, pr. aconstructor.
-  apply vsubtype_refl. inv p. inv H0. auto.
-+ inv H0. eapply inv_ann_Right in H.
-  destruct H as [v1'[B'[p1[styb othr]]]].
-  exists v1',B',p1. aconstructor.
-  eapply vsubtype_trans; eauto.
-Qed.
-
-Fixpoint inv_ann_Nil Γ A p v'
-  (ann: v_ann Γ Nil A p v') {struct ann}:
-  v' = SkNil.
-Proof.
-inv ann. auto.
-eapply inv_ann_Nil in H. auto.
-Qed.
-
-Fixpoint inv_ann_Cons Γ v1 v2 A p v'
-  (ann: v_ann Γ (Cons v1 v2) (TyList A) p v') {struct ann}:
-  exists v1' v2' A' p1 p2,
-    vsubtype A' A /\
-    v_ann Γ v1 A' p1 v1' /\ v_ann Γ v2 (TyList A') p2 v2' /\
-    v' = SkCons v1' v2'.
-Proof.
-inv ann.
-+ exists v1', v2', A, p1, p2. aconstructor.
-  all: apply vsubtype_refl; inv p; inv H0; auto.
-+ inv H0. eapply inv_ann_Cons in H.
-  destruct H as [v1'[v2'[A'[p1[p2[stya othr]]]]]].
-  exists v1',v2',A',p1,p2.
-  aconstructor. eapply vsubtype_trans; eauto.
-Qed.
-
-Fixpoint inv_ann_Fun Γ c A C p v'
-  (ann: v_ann Γ (Fun c) (TyFun A C) p v') {struct ann}:
-  exists c' A' C' p1,
-    vsubtype A A' /\ csubtype C' C /\
-    c_ann (CtxU Γ A') c C' p1 c' /\
-    v' = SkFun c'.
-Proof.
-inv ann.
-+ exists c', A, C, pc. do 2 try aconstructor.
-  all: apply vsubtype_refl || apply csubtype_refl ; inv p; inv H0; auto.
-+ inv H0. eapply inv_ann_Fun in H.
-  destruct H as [c'[A'[C'[p1[stya[styc othr]]]]]].
-  exists c',A',C',p1.
-  do 2 try aconstructor. eapply vsubtype_trans; eauto.
-  eapply csubtype_trans; eauto.
-Qed.
-
-Fixpoint inv_ann_Handler Γ c h C D p v'
-  (ann: v_ann Γ (Handler c h) (TyHandler C D) p v') {struct ann}:
-  exists c' h' A' Σ' E' D' pc ph,
-    csubtype C (CTy A' Σ' E') /\ csubtype D' D /\
-    c_ann (CtxU Γ A') c D' pc c' /\
-    h_ann Γ h Σ' D' ph h' /\
-    v' = SkHandler c' h'.
-Proof.
-inv ann.
-+ exists c', h', A, Σ, E, D, pc, ph. aconstructor. 2: aconstructor.
-  all: apply csubtype_refl ; inv p; inv H0; auto.
-+ inv H0. eapply inv_ann_Handler in H. clear inv_ann_Handler.
-  destruct H as [c'[h'[A'[Σ'[E'[D'[pc[ph[styc[styd othr]]]]]]]]]].
-  exists c',h',A',Σ',E',D',pc,ph.
-  do 2 try aconstructor. all: eapply csubtype_trans; eauto.
-Qed.
-
-(* Inversions for computations *)
-
-Fixpoint inv_ann_Ret Γ v A Σ E p csk
-  (ann: c_ann Γ (Ret v) (CTy A Σ E) p csk) {struct ann}:
-  exists v' A' p',
-    vsubtype A' A /\ v_ann Γ v A' p' v' /\ csk = SkRet v'.
-Proof.
-inv ann.
-+ exists v', A, pv. aconstructor.
-  apply vsubtype_refl. inv p. inv H0. auto.
-+ inv H0. eapply inv_ann_Ret in H.
-  destruct H as [v1'[A'[p1[stya othr]]]].
-  exists v1',A',p1. aconstructor.
-  eapply vsubtype_trans; eauto.
-Qed.
-
-Fixpoint inv_ann_Absurd Γ v C p csk
-  (ann: c_ann Γ (Absurd v) C p csk) {struct ann}:
-  exists v' p',
-    v_ann Γ v TyEmpty p' v' /\ csk = SkAbsurd v'.
-Proof.
-inv ann.
-+ exists v', pv. aconstructor.
-+ inv H0. eapply inv_ann_Absurd in H.
-  destruct H as [v1'[p1[ty othr]]].
-  exists v1', p1. aconstructor.
-Qed.
-
-Fixpoint inv_ann_ProdMatch Γ v c C p csk
-  (ann: c_ann Γ (ProdMatch v c) C p csk) {struct ann}:
-  exists v' A B pv c' C' pc,
-    v_ann Γ v (TyProd A B) pv v' /\ c_ann (CtxU (CtxU Γ A) B) c C' pc c'
-    /\ csubtype C' C /\ csk = SkProdMatch v' c'.
-Proof.
-inv ann.
-+ exists v', A, B, pv, c', C, pc. do 3 try aconstructor.
-  apply csubtype_refl. inv p. auto.
-+ eapply inv_ann_ProdMatch in H. clear inv_ann_ProdMatch.
-  destruct H as [v'[A[B[pv[c'[C'[pc othr]]]]]]].
-  destruct othr as [vann[cann[csty id]]].
-  subst.
-  exists v', A, B, pv, c', C', pc.
-  do 3 try aconstructor. eapply csubtype_trans; eauto.
-Qed.
-
-
-Fixpoint inv_ann_SumMatch Γ v c1 c2 C p csk
-  (ann: c_ann Γ (SumMatch v c1 c2) C p csk) {struct ann}:
-  exists v' A B pv c1' c2' C' pc1 pc2,
-    v_ann Γ v (TySum A B) pv v' /\ c_ann (CtxU Γ A) c1 C' pc1 c1'
-    /\ c_ann (CtxU Γ B) c2 C' pc2 c2'
-    /\ csubtype C' C /\ csk = SkSumMatch v' c1' c2'.
-Proof.
-inv ann.
-+ exists v', A, B, pv, c1', c2', C, pc1, pc2. do 4 try aconstructor.
-  apply csubtype_refl. inv p. auto.
-+ eapply inv_ann_SumMatch in H. clear inv_ann_SumMatch.
-  destruct H as [v'[A[B[pv[c1'[c2'[C'[pc1[pc2 othr]]]]]]]]].
-  destruct othr as [vann[cann1[cann2[csty id]]]].
-  subst.
-  exists v', A, B, pv, c1', c2', C', pc1, pc2.
-  do 4 try aconstructor. eapply csubtype_trans; eauto.
-Qed.
-
-Fixpoint inv_ann_ListMatch Γ v c1 c2 C p csk
-  (ann: c_ann Γ (ListMatch v c1 c2) C p csk) {struct ann}:
-  exists v' A pv c1' c2' C' pc1 pc2,
-    v_ann Γ v (TyList A) pv v' /\ c_ann Γ c1 C' pc1 c1'
-    /\ c_ann (CtxU (CtxU Γ A) (TyList A)) c2 C' pc2 c2'
-    /\ csubtype C' C /\ csk = SkListMatch v' c1' c2'.
-Proof.
-inv ann.
-+ exists v', A, pv, c1', c2', C, pc1, pc2. do 4 try aconstructor.
-  apply csubtype_refl. inv p. auto.
-+ eapply inv_ann_ListMatch in H. clear inv_ann_ListMatch.
-  destruct H as [v'[A[pv[c1'[c2'[C'[pc1[pc2 othr]]]]]]]].
-  destruct othr as [vann[cann1[cann2[csty id]]]].
-  subst.
-  exists v', A, pv, c1', c2', C', pc1, pc2.
-  do 4 try aconstructor. eapply csubtype_trans; eauto.
-Qed.
-
-Fixpoint inv_ann_Op Γ id v c C p c'
-  (ann: c_ann Γ (Op id v c) C p c') {struct ann}:
-  exists vop' cop' Aop' Bop' A' Σ' E' p1 p2,
-    csubtype (CTy A' Σ' E') C /\
-    get_op_type Σ' id = Some (Aop', Bop') /\
-    v_ann Γ v Aop' p1 vop' /\ c_ann (CtxU Γ Bop') c (CTy A' Σ' E') p2 cop' /\
-    c' = SkOp id (skeletize_vtype Aop') (skeletize_vtype Bop') vop' cop'.
-Proof.
-inv ann.
-+ exists v', c'0, Aop, Bop, A, Σ, E, pv, pc. do 2 try aconstructor.
-  all: apply vsubtype_refl || apply sig_subtype_refl || eapply eqs_subtype_refl.
-  all: inv p; inv H0; eauto.
-+ destruct C as [a σ e]. inv H0.
-  eapply shape_op_full in p' as shape. 2: reflexivity. 2: reflexivity.
-  destruct shape as [Aop'[Bop'[gets' _]]]. 
-  eapply inv_ann_Op in H. clear inv_ann_Op.
-  destruct H as [vop'[cop'[Aop''[Bop''[A''[Σ''[E'' othr]]]]]]].
-  destruct othr as [p1[p2[styc[gets''[ann1[ann2 s']]]]]].
-  subst. inv styc.
-  exists vop', cop', Aop'', Bop'', A'', Σ'', E'', p1, p2.
-  do 2 try aconstructor.
-  - eapply vsubtype_trans; eauto.
-  - eapply sig_subtype_trans; eauto.
-  - eapply eqs_subtype_trans; eauto.
-Qed.
-
-
-
-(* Show uniqueness *)
-(* We are lucky because there are no restrictions on the context! <3 *)
-
-Fixpoint v_ann_unique Γ1 Γ2 v A A1 A2 v1 v2
-  (tys1: has_vtype Γ1 v A1) (tys2: has_vtype Γ2 v A2)
-  (ann1: v_ann Γ1 v A1 tys1 v1) (ann2: v_ann Γ2 v A2 tys2 v2) {struct ann1}:
-  vsubtype A1 A -> vsubtype A2 A ->
-  v1 = v2
-
-with c_ann_unique Γ1 Γ2 c C C1 C2 c1 c2
-  (tys1: has_ctype Γ1 c C1) (tys2: has_ctype Γ2 c C2)
-  (ann1: c_ann Γ1 c C1 tys1 c1) (ann2: c_ann Γ2 c C2 tys2 c2) {struct ann1}:
-  csubtype C1 C -> csubtype C2 C ->
-  c1 = c2
-
-with h_ann_unique Γ1 Γ2 h Σ1 Σ2 D D1 D2 h1 h2
-  (tys1: has_htype Γ1 h Σ1 D1) (tys2: has_htype Γ2 h Σ2 D2)
-  (ann1: h_ann Γ1 h Σ1 D1 tys1 h1) (ann2: h_ann Γ2 h Σ2 D2 tys2 h2) {struct ann1}:
-  csubtype D1 D -> csubtype D2 D ->
-  h1 = h2.
-
-Proof.
-all: rename v_ann_unique into VL.
-all: rename c_ann_unique into CL.
-all: rename h_ann_unique into HL.
-{
-intros sty1 sty2. destruct ann1.
-Focus 11. (* Subtyping on left *)
-  eapply VL. eauto. eauto. 2: eauto.
-  eapply vsubtype_trans. all: eauto.
-
-+ eapply inv_ann_Var in ann2; eauto.
-+ apply inv_ann_Unit in ann2; auto.
-+ eapply inv_ann_Int in ann2; eauto.
-+ eapply shape_pair_full in tys2 as shape. 2: reflexivity.
-  destruct shape as [A'[B'[s[t1 t2]]]]. subst.
-  apply inv_ann_Pair in ann2.
-  destruct ann2 as [v1''[v2''[A''[B''[p1''[p2'' othr]]]]]].
-  destruct othr as [stya[styb[ann2_1[ann2_2 id]]]].
-  subst. f_equal. 
-  - inv sty1. inv sty2. eapply VL; eauto.
-    eapply vsubtype_trans; eauto.
-  - inv sty1. inv sty2. eapply VL; eauto. 
-    eapply vsubtype_trans; eauto.
-+ eapply shape_left_full in tys2 as shape. 2: reflexivity.
-  destruct shape as [A'[B'[s t]]]. subst.
-  apply inv_ann_Left in ann2.
-  destruct ann2 as [v''[A''[p''[stya[ann2 id]]]]].
-  subst. f_equal.
-  inv sty1. eapply VL; eauto. inv sty2.
-  eapply vsubtype_trans; eauto.
-+ eapply shape_right_full in tys2 as shape. 2: reflexivity.
-  destruct shape as [A'[B'[s t]]]. subst.
-  apply inv_ann_Right in ann2.
-  destruct ann2 as [v''[B''[p''[styb[ann2 id]]]]].
-  subst. f_equal.
-  inv sty1. eapply VL; eauto. inv sty2.
-  eapply vsubtype_trans; eauto.
-+ eapply inv_ann_Nil in ann2. auto.
-+ eapply shape_cons_full in tys2 as shape. 2: reflexivity.
-  destruct shape as [A'[s[t1 t2]]]. subst.
-  apply inv_ann_Cons in ann2.
-  destruct ann2 as [v1''[v2''[A''[p1''[p2''[stya[t1'[t2' id]]]]]]]].
-  subst. f_equal.
-  - inv sty1. inv sty2. eapply VL; eauto.
-    eapply vsubtype_trans; eauto.
-  - inv sty1. inv sty2. eapply VL; eauto.
-    all: apply STyList. eauto. eapply vsubtype_trans; eauto.
-+ eapply shape_fun_full in tys2 as shape. 2: reflexivity.
-  destruct shape as [A'[C'[s t]]]. subst.
-  apply inv_ann_Fun in ann2.
-  destruct ann2 as [c''[A''[C''[p''[stya[styc[ann2 id]]]]]]].
-  subst. f_equal.
-  inv sty1. inv sty2. eapply CL; eauto.
-  eapply csubtype_trans; eauto.
-+ eapply shape_handler_full in tys2 as shape. 2: reflexivity.
-  destruct shape as [A'[Σ'[E'[D'[Σ''[D''[s[ct[ht[r[ssty csty]]]]]]]]]]]. subst.
-  apply inv_ann_Handler in ann2.
-  destruct ann2 as [c''[h''[A'''[Σ'''[E'''[D'''[pc'[ph' othr]]]]]]]].
-  destruct othr as [csty'[dsty'[cann[hann s]]]].
-  subst. f_equal.
-  - inv sty1. inv sty2. inv H3. inv H6. eapply CL; eauto.
-    eapply csubtype_trans; eauto.
-  - inv sty1. inv sty2. inv H3. inv H6. eapply HL; eauto. 
-    eapply csubtype_trans; eauto.
-}{
-intros sty1 sty2. clear HL. destruct ann1.
-Focus 11. (* Subtyping on left *)
-  eapply CL. eauto. eauto. 2: eauto.
-  eapply csubtype_trans. all: eauto.
-
-+ destruct C2 as [A2 Σ2 E2].
-  eapply shape_ret_full in tys2 as shape. 2: reflexivity. 2: reflexivity.
-  apply inv_ann_Ret in ann2.
-  destruct ann2 as [v''[A''[p''[stya[ann2 id]]]]].
-  subst. f_equal.
-  inv sty1. eapply VL; eauto. inv sty2.
-  eapply vsubtype_trans; eauto.
-+ eapply shape_absurd_full in tys2 as shape. 2: reflexivity.
-  apply inv_ann_Absurd in ann2.
-  destruct ann2 as [v''[p''[ann2 id]]].
-  subst. f_equal.
-  inv sty1. eapply VL; eauto; apply STyEmpty.
-+ eapply inv_ann_ProdMatch in ann2.
-  destruct ann2 as [v''[A'[B'[pv'[c''[C'[pc' othr]]]]]]].
-  destruct othr as [vann[cann[csty id]]].
-  subst. f_equal.
-  - eapply VL; eauto.
-+ admit.
-+ admit.
-+ admit.
-+ admit.
-+ admit.
-+ admit.
-+ destruct C2 as [A2 Σ2 E2].
-  eapply shape_op_full in tys2 as shape; try reflexivity.
-  destruct shape as [Aop'[Bop'[gets'[vty' cty']]]].
-  eapply inv_ann_Op in ann2.
-  destruct ann2 as [vop'[cop'[Aop''[Bop''[A''[Σ''[E'' othr]]]]]]].
-  destruct othr as [p1[p2[styc[gets''[vann2[cann2 s]]]]]].
-  inv sty1. inv sty2.
-  assert (sig_subtype Σ'' Σ') as stytrans.
-  { inv styc. eapply sig_subtype_trans; eauto. }
-  eapply sig_subtype_get_Some in stytrans as styop. 2: eauto.
-  destruct styop as [a[b[sget1[sa sb]]]].
-  eapply sig_subtype_get_Some in H6 as styop. 2: eauto.
-  destruct styop as [a'[b'[sget2[sa' sb']]]].
-  rewrite sget2 in sget1. inv sget1. clear sget2.
-  subst. f_equal.
-  - clear VL CL.
-    apply skeletons_ignore_vsubtype in sa. rewrite sa. clear sa.
-    apply skeletons_ignore_vsubtype. auto.
-  - clear VL CL.
-    apply skeletons_ignore_vsubtype in sb. rewrite <-sb. clear sb.
-    symmetry. apply skeletons_ignore_vsubtype. auto.
-  - eapply VL; eauto.
-  - eapply CL. eauto. eauto.
-    eapply STyCTy; eauto.
-    eapply csubtype_trans; eauto. eapply STyCTy; eauto.
-}{
-intros csty1 csty2. clear VL. destruct ann1.
-inv ann2. auto.
-inv ann2. f_equal.
-+ clear CL. eapply HL; eauto; clear HL.
-+ clear HL. eapply CL; eauto.
-}
-Admitted.
-
-
-Fixpoint v_ann_unique_clean Γ v A v1 v2 
-  (tys1: has_vtype Γ v A) (tys2: has_vtype Γ v A)
-  (ann1: v_ann Γ v A tys1 v1) (ann2: v_ann Γ v A tys2 v2):
-  v1 = v2
-
-with c_ann_unique_clean Γ c C c1 c2
-  (tys1: has_ctype Γ c C) (tys2: has_ctype Γ c C)
-  (ann1: c_ann Γ c C tys1 c1) (ann2: c_ann Γ c C tys2 c2):
-  c1 = c2
-
-with h_ann_unique_clean Γ h Σ D h1 h2
-  (tys1: has_htype Γ h Σ D) (tys2: has_htype Γ h Σ D)
-  (ann1: h_ann Γ h Σ D tys1 h1) (ann2: h_ann Γ h Σ D tys2 h2):
-  h1 = h2.
-
-Proof.
-+ eapply v_ann_unique; eauto.
-  all: apply vsubtype_refl; clear ann1; inv tys1; auto.
-+ eapply c_ann_unique; eauto.
-  all: apply csubtype_refl; clear ann1; inv tys1; auto.
-+ eapply h_ann_unique; eauto.
-  all: apply csubtype_refl; clear ann1; inv tys1; auto.
-Qed.
